lib/Benchmarks/MPLSVectorizedProof.v
@@ -1,10 +1,11 @@
 Require Import Leapfrog.Benchmarks.ProofHeader.
 Require Import Leapfrog.Benchmarks.MPLSVectorized. 
+Require Import Leapfrog.FirstOrderConfRelSimplified.
 
 Ltac compile_fm H el er :=
-  time "compilation correct" erewrite compilation_corr with (St1_eq_dec := el) (St2_eq_dec := er) in H.
-  
-  (* ;
+  time "compilation correct" erewrite compilation_corr with (St1_eq_dec := el) (St2_eq_dec := er) in H; [
+    | typeclasses eauto | typeclasses eauto | eapply check_fm_wf_corr; exact eq_refl
+  ];
   simpl in H;
   (* these could be invariants and somehow avoided completely
       or if they have to be done it could all be done with reflection *)
@@ -18,7 +19,7 @@ Ltac compile_fm H el er :=
     ]
 
   end;
-  crunch_foterm_ctx. *)
+  crunch_foterm_ctx.
 
 Ltac decide_entailment H P HP el er P_orig e :=
   let Horig := fresh "Horig" in
@@ -26,21 +27,19 @@ Ltac decide_entailment H P HP el er P_orig e :=
   time "remembering iff" remember_iff P HP e;
   time "Horig" assert (Horig: P_orig <-> P)
     by (rewrite HP; eapply iff_refl);
-  time "compile fm" compile_fm HP el er.
-
-(*   
+  time "compile fm" compile_fm HP el er;
   match goal with
   | HP: P <-> interp_fm ?v ?f |- _ =>
       time "smt check neg" check_interp_neg (interp_fm v f);
       idtac "UNSAT";
       time "asserting neg" assert (~ P_orig) by (rewrite -> Horig; rewrite -> HP; apply dummy_pf_false)
   | HP: P <-> interp_fm ?v ?f |- _ =>
-      time "smt check pos" check_interp_pos (interp_fm v f);
+     time "smt check pos" check_interp_pos (interp_fm v f);
       idtac "SAT";
       time "asserting pos" assert (P_orig) by (rewrite -> Horig; rewrite -> HP; apply dummy_pf_true)
   | |- _ => idtac "undecided goal :("
   end;
-  time "clearing Horig" clear Horig. *)
+  time "clearing Horig" clear Horig.
 
 Ltac run_bisim_axiom el er use_hc :=
   match goal with
@@ -54,15 +53,14 @@ Ltac run_bisim_axiom el er use_hc :=
                                                             top' _ _ _ _ _ r_states
                                                                  (conf_to_state_template q1)
                                                                  (conf_to_state_template q2))
-                                                         ({| e_prem := R; e_concl := C |}))
-                                                         (* ;
-      match goal with
+                                                         ({| e_prem := R; e_concl := C |}));
+      match goal with 
       | HN: ~ P_orig |- _ =>
           time "extending" (extend_bisim' HN use_hc; clear HN)
       | H: P_orig |- pre_bisimulation _ _ _ _ (?C :: _) _ _ =>
           time "skipping" (skip_bisim' H; clear H; try clear C)
       end;
-      time "clearing all" clear P HP P_orig *)
+      time "clearing all" clear P HP P_orig
   end.
 
 Ltac solve_lang_equiv_state_axiom el er use_hc :=
@@ -78,8 +76,6 @@ Ltac solve_lang_equiv_state_axiom el er use_hc :=
   time "close phase" close_bisim_axiom. *)
 
 
-  
-
 Lemma mpls_equiv:
   lang_equiv_state
     (P4A.interp Plain.aut)
@@ -89,6 +85,21 @@ Lemma mpls_equiv:
 Proof.
 
   time "mpls no hc" solve_lang_equiv_state_axiom Plain.state_eqdec Unrolled.state_eqdec false.
+
+
+  4: {
+    eapply check_fm_wf_corr;
+    exact eq_refl.
+    3: {
+      exact (@Sum.sum Plain.state Unrolled.state Plain.header Plain.sz
+      Unrolled.header Unrolled.sz Plain.aut Unrolled.aut).
+    }
+    3: 
+    4: exact eq_refl.
+    all: typeclasses eauto.
+    exact eq_refl.
+    
+  }
   (* time "mpls hc" solve_lang_equiv_state_axiom Plain.state_eqdec Unrolled.state_eqdec true. *)
 
 Time Qed.
